Weidenbach_Book/IsaSAT/IsaSAT_Stats_LLVM.thy
@@ -2,8 +2,6 @@ theory IsaSAT_Stats_LLVM
 imports IsaSAT_Stats IsaSAT_EMA_LLVM IsaSAT_Rephase_LLVM IsaSAT_Reluctant_LLVM Tuple16_LLVM
 begin
 
-no_notation WB_More_Refinement.fref (\<open>[_]\<^sub>f _ \<rightarrow> _\<close> [0,60,60] 60)
-no_notation WB_More_Refinement.freft (\<open>_ \<rightarrow>\<^sub>f _\<close> [60,60] 60)
 hide_const (open) NEMonad.RETURN NEMonad.ASSERT
 
 
